snap

iocy/FancyTraces2.fst
@@ -3,31 +3,95 @@ module FancyTraces2
 open FStar.List.Tot
 open FStar.Ghost
 
+module FSet = FStar.FiniteSet.Base
 module M = FStar.FiniteMap.Base
 
 type promise_id = nat
 
 noeq
-type promise (e:Type u#a) (a:Type u#b) : Type u#(max a b) =
-| Promise : id:promise_id -> r:erased a -> promise e a
+type promise (e:Type u#0) (a:Type u#0) : Type u#0 =
+| Promise : id:promise_id -> promise e a
 (** CA: having the local trace on the promise, pushes the promise type to universe 1, preventing HO promises **)
 
-let suffix_of l h = admit ()
-let lemma_suffix_of_reflexive l = admit ()
-
-type parallel_traces e : Type u#1 = (* promise_id -> atrace *)
-  M.map promise_id (atrace e)
-  (* CA: this nat should be promise_id, but is not an eqtype? *)
+type parallel_traces (e:Type0) : Type u#1 = (* promise_id -> atrace *)
+  n:nat & m:(M.map promise_id (a:Type0 & a & atrace e)){
+    forall id. id `FSet.mem` (M.domain m) <==> id < n
+  }
   // M.map int (a:Type0 & pr:promise e a & tr:atrace e)
   (* CA: why do I have the promise here? *)
 
-let mem_id (id:promise_id) (pts:parallel_traces 'e) = reveal id `M.mem` pts
-let sel_id (id:promise_id) (pts:(parallel_traces 'e){id `mem_id` pts}) : (atrace 'e) =
-  M.lookup id pts
+let mem_id (id:promise_id) (pts:parallel_traces 'e) = id `M.mem` (dsnd pts)
+let sel_id (id:promise_id) (pts:(parallel_traces 'e){id `mem_id` pts}) : a:Type0 & a & atrace 'e =
+  M.lookup id (dsnd pts)
   // Mkdtuple3?._3 (M.lookup id pts)
 
-let mem (pr:promise 'e 'a) (pts:parallel_traces 'e) = pr.id `mem_id` pts
-let sel (pr:promise 'e 'a) (pts:(parallel_traces 'e){pr `mem` pts}) :  atrace 'e =
-  sel_id pr.id pts
-let insert (pr:promise 'e 'a) (lt:atrace 'e) (pts:parallel_traces 'e) : parallel_traces 'e =
-  M.insert pr.id lt pts
+let mem (pr:promise 'e 'a) (pts:parallel_traces 'e) = pr.id `mem_id` pts /\ 'a == (sel_id pr.id pts)._1
+
+let sel_lt pr pts = (sel_id pr.id pts)._3
+let sel_r pr pts = (sel_id pr.id pts)._2
+let sel_a pr pts = (sel_id pr.id pts)._1
+
+let async r lt pts =
+  let (| n, m |) = pts in
+  let m' = M.insert (n+1) (| _, r, lt |) m in
+  admit ();
+  let pts' : parallel_traces _ = (| n + 1, m' |) in
+  (Promise (n+1), pts')
+
+let await pr pts =
+  let (| n, m |) = pts in
+  let m' = M.insert pr.id (| _, sel_r pr pts, [] |) m in
+  admit ();
+  (| n, m' |)
+
+let closed_atrace pts tr = admit ()
+let closed_atrace_async h pts r lt = admit ()
+let closed_atrace_await_pr pr h pt = admit ()
+let closed_atrace_produce ev h pts = admit ()
+
+let size_pts pr = admit ()
+
+let fulfilled pr pts : bool =
+  match sel_lt pr pts with
+  | [] -> true
+  | _ -> false
+
+let waiting pr pts : bool =
+  match sel_lt pr pts with
+  | EAwait _::_ -> true
+  | _ -> false
+
+let can_progress pr pts =
+  not (fulfilled pr pts) && not (waiting pr pts)
+
+let generate_all_promises #e pts : list (a:Type0 & pr:promise e a{pr `mem` pts}) =
+  let (| n, m |) = pts in
+  let rec aux (i:nat{i < n}) : list (a:Type0 & pr:promise e a{pr `mem` pts}) = begin
+    let pr : promise e (sel_id i pts)._1 = Promise i in
+    if i = 0 then [(| _, pr |)]
+    else ([(| _, pr |)] @ aux (i-1))
+  end in
+  if 0 < n then aux (n-1)
+  else []
+
+
+let get_next #e pts =
+  let l = filter (fun (apr:(a:Type0 & pr:promise e a{pr `mem` pts})) -> can_progress (dsnd apr) pts) (generate_all_promises pts) in
+  admit ();
+  l
+
+let simple_progress (pr:promise 'e 'a) (pts:(parallel_traces 'e){pr `mem` pts /\ can_progress pr pts})
+  : 'e * pts':parallel_traces 'e{size_pts pts' < size_pts pts} =
+  let (| n, m |) = pts in
+  match sel_lt pr pts with
+  | ev :: tl -> begin
+    let m' = M.insert pr.id (| _, sel_r pr pts, tl |) m in
+    admit ();
+    (ev, (| n, m' |))
+  end
+
+(**
+let normalize (pts:parallel_traces 'e) : parallel_traces 'e =
+  let l = filter (fun (apr:(a:Type0 & pr:promise e a{pr `mem` pts})) -> can_progress (dsnd apr) pts) (generate_all_promises pts) in **)
+
+let progress pr pts = admit ()
